src/SDK/Materials.dfy
@@ -27,20 +27,14 @@ module Materials {
       |providerInfo| < UINT16_LIMIT &&
       |ciphertext| < UINT16_LIMIT
     }
+
+    static function method ValidWitness(): EncryptedDataKey {
+      EncryptedDataKey("provider", StringToByteSeq("provider info"), StringToByteSeq("cypher text"))
+    }
   }
 
   // TODO: Add keyring trace
-  datatype EncryptionMaterialsInput = EncryptionMaterialsInput(algorithmSuiteID: AlgorithmSuite.ID,
-                                                               encryptionContext: EncryptionContext,
-                                                               plaintextDataKey: Option<seq<uint8>>) 
-  {
-    predicate Valid() {
-      (plaintextDataKey.None? || algorithmSuiteID.ValidPlaintextDataKey(plaintextDataKey.get))
-    }
-  }
-  type ValidEncryptionMaterialsInput = i: EncryptionMaterialsInput | i.Valid() witness EncryptionMaterialsInput(0x0014, [], None)
-
-  datatype DataKey = DataKey(algorithmSuiteID: AlgorithmSuite.ID, // TODO-RS: This could be a ghost var?
+  datatype DataKey = DataKey(algorithmSuiteID: AlgorithmSuite.ID,
                              plaintextDataKey: seq<uint8>,
                              encryptedDataKeys: seq<EncryptedDataKey>) 
   {
@@ -48,12 +42,16 @@ module Materials {
       algorithmSuiteID.ValidPlaintextDataKey(plaintextDataKey)
       // TODO-RS: assert that the encrypted data keys are actually tied to the plaintext!
     }
+
+    static function method ValidWitness(): DataKey { 
+      DataKey(AlgorithmSuite.AES_256_GCM_IV12_TAG16_HKDF_SHA384_ECDSA_P384, 
+              seq(32, i => 0), 
+              [EncryptedDataKey.ValidWitness()])
+    }
   }
 
-  function method ValidDataKeyWitness(): DataKey { 
-    DataKey(AlgorithmSuite.AES_256_GCM_IV12_TAG16_HKDF_SHA384_ECDSA_P384, seq(32, i => 0), [])
-  }  
-  type ValidDataKey = i: DataKey | i.Valid() witness ValidDataKeyWitness()
+    
+  type ValidDataKey = i: DataKey | i.Valid() witness DataKey.ValidWitness()
 
   predicate method CompatibleDataKeys(k1: ValidDataKey, k2: ValidDataKey) {
     k1.algorithmSuiteID == k2.algorithmSuiteID && k1.plaintextDataKey == k2.plaintextDataKey
@@ -69,69 +67,20 @@ module Materials {
     r
   }
 
-  predicate method ValidOnEncryptResult(input: ValidEncryptionMaterialsInput, output: ValidDataKey) {
-    input.algorithmSuiteID == output.algorithmSuiteID &&
-    input.plaintextDataKey.Some? ==> input.plaintextDataKey.get == output.plaintextDataKey
-  }
-
-  lemma ValidOnEncryptResultImpliesSameAlgorithmSuiteID(input: ValidEncryptionMaterialsInput, output: ValidDataKey) 
-    requires ValidOnEncryptResult(input, output)
-    ensures input.algorithmSuiteID == output.algorithmSuiteID
-  {}
-
-  lemma MergingResults(input: ValidEncryptionMaterialsInput, dk1: ValidDataKey, dk2: ValidDataKey) 
-    requires ValidOnEncryptResult(input, dk1)
-    requires ValidOnEncryptResult(input, dk2)
-    requires dk1.plaintextDataKey == dk2.plaintextDataKey
-    ensures CompatibleDataKeys(dk1, dk2)
-    ensures ValidOnEncryptResult(input, MergeDataKeys(dk1, dk2)) 
-  {
-    ValidOnEncryptResultImpliesSameAlgorithmSuiteID(input, dk1);
-    ValidOnEncryptResultImpliesSameAlgorithmSuiteID(input, dk2);
-    assert input.algorithmSuiteID == dk1.algorithmSuiteID == dk2.algorithmSuiteID;
-    if (input.plaintextDataKey.Some?) {
-      assert input.plaintextDataKey.get == dk1.plaintextDataKey == dk2.plaintextDataKey;
-    }
-  }
-
-  datatype EncryptionMaterialsOutput = EncryptionMaterialsOutput(dataKey: ValidDataKey,
-                                                                 signingKey: Option<seq<uint8>>)
+  datatype EncryptionMaterials = EncryptionMaterials(dataKey: ValidDataKey,
+                                                     signingKey: Option<seq<uint8>>)
   {
     predicate method Valid() {
       && dataKey.algorithmSuiteID.SignatureType().Some? ==> signingKey.Some?
-      // TODO-RS:
-      // && |dataKey.encryptedDataKeys| > 0
+      && |dataKey.encryptedDataKeys| > 0
     }
   }
-  type ValidEncryptionMaterialsOutput = i: EncryptionMaterialsOutput | i.Valid() 
-    witness EncryptionMaterialsOutput(ValidDataKeyWitness(), Some(seq(32, i => 0)))
+  type ValidEncryptionMaterials = i: EncryptionMaterials | i.Valid() 
+    witness EncryptionMaterials(DataKey.ValidWitness(), Some(seq(32, i => 0)))
 
   // TODO: Add keyring trace
-  datatype DecryptionMaterialsOutput = DecryptionMaterialsOutput(dataKey: ValidDataKey,
-                                                                 verificationKey: Option<seq<uint8>>)
-  {
-    predicate method Valid() {
-      dataKey.algorithmSuiteID.SignatureType().Some? ==> verificationKey.Some?
-    }
-  }
-  type ValidDecryptionMaterialsOutput = i: DecryptionMaterialsOutput | i.Valid() 
-    witness DecryptionMaterialsOutput(ValidDataKeyWitness(), Some(seq(32, i => 0)))
-
-  predicate method ValidOnDecryptResult(algorithmSuiteID: AlgorithmSuite.ID, 
-                                        encryptionContext: EncryptionContext, 
-                                        edks: seq<EncryptedDataKey>, 
-                                        output: ValidDataKey) {
-    && output.algorithmSuiteID == algorithmSuiteID
-    && output.encryptedDataKeys == edks
-  }
-
-  lemma ValidOnDecryptResultImpliesSameAlgorithmSuiteID(algorithmSuiteID: AlgorithmSuite.ID, 
-                                                        encryptionContext: EncryptionContext, 
-                                                        edks: seq<EncryptedDataKey>, 
-                                                        output: ValidDataKey)
-    requires ValidOnDecryptResult(algorithmSuiteID, encryptionContext, edks, output)
-    ensures output.algorithmSuiteID == algorithmSuiteID
-  {}
+  datatype DecryptionMaterials = DecryptionMaterials(plaintextDataKey: seq<uint8>,
+                                                     verificationKey: Option<seq<uint8>>)
 
     //TODO: Review this code.
     function method naive_merge<T> (x : seq<T>, y : seq<T>, lt : (T, T) -> bool) : seq<T>
